Projects/AP/Alts/Alt1/Equiv.lean
@@ -125,11 +125,11 @@ theorem Game.not_dWinsAt_iff {pw} {g : Game pw} : ¬g.DWins ↔ g.AWins := by
 theorem dMoveValid_none {b : Board} : DMoveValid b none := by
   simp [DMoveValid]
 
-@[instance]
+@[simp, instance]
 theorem A.nonempty {pw} : Nonempty (A pw) :=
   ⟨⟨λ _ _ h => ⟨_, h.choose_spec⟩⟩⟩
 
-@[instance]
+@[simp, instance]
 theorem D.nonempty : Nonempty D :=
   ⟨⟨λ _ _ => ⟨none, by simp⟩⟩⟩
 
@@ -150,7 +150,7 @@ instance : Inhabited Board := ⟨board₀⟩
 instance : Inhabited State := ⟨state₀⟩
 
 @[simp]
-theorem toAltH_state₀_eq {pw} : state₀.toAltH pw = AP.initState pw 0 := by
+theorem toAltH_state₀ {pw} : state₀.toAltH pw = AP.initState pw 0 := by
   simp [State.toAltH, State.toAltH?, Board.toAltH?]
   apply choose?_of_pos (P := λ (s : Option AP.State) => s.getd = _) _ _
   · use AP.initState pw 0; simp
@@ -158,8 +158,8 @@ theorem toAltH_state₀_eq {pw} : state₀.toAltH pw = AP.initState pw 0 := by
   rw [State.hist_eq_aPos_of] <;> rw [←h₂] <;> simp
 
 @[simp]
-theorem toAltH_board₀_eq {pw} : board₀.toAltH pw false = AP.initState pw 0 :=
-  toAltH_state₀_eq
+theorem toAltH_board₀ {pw} : board₀.toAltH pw false = AP.initState pw 0 :=
+  toAltH_state₀
 
 @[simp, instance]
 theorem initial_toAltH_state₀ {pw} : sys.Initial # state₀.toAltH pw := by
@@ -197,6 +197,7 @@ theorem act_state₀ : state₀.act := trivial
 
 theorem State.dwn_eq {pw} {s : State} : s.dwn pw = (s.toAltH pw).dwn := rfl
 
+@[simp]
 theorem Game.play_succ {pw} {g : Game pw} {n} : g.play (n + 1) = (g.play n).playMove := by
   rw [play, Function.iterate_succ']; rfl
 
@@ -285,10 +286,6 @@ theorem State.wf_iff {pw} {s : State} : s.WF pw ↔ ∃ a d n g,
 (initGame a d state₀ : Game pw).play n = g ∧ (g.s = s ∨ ∃ h, (playDMoveAt g h).s = s) :=
   ⟨λ ⟨h⟩ => h, λ h => ⟨h⟩⟩
 
-@[simp, instance]
-theorem wf_state₀ {pw} : state₀.WF pw := by
-  rw [State.wf_iff]; use default, default, 0; simp
-
 @[simp]
 theorem Game.setState_initGame {pw a d s s'} :
 (initGame a d s : Game pw).setState s' = initGame a d s' := rfl
@@ -331,6 +328,11 @@ theorem Game.act_play_initGame_of_not_aTurn {pw a d n g s}
   have H₂ : s₁.aTurn = true; simpa [←h₅]
   have H₃ : s₂.aTurn = false; simpa [←hs₂]
   grind
+
+@[simp]
+theorem Game.s_playAMoveAt'_eq_iff {pw} {g₁ g₂ : Game pw} {h₁ h₂ h₃ h₄} :
+(playAMoveAt' g₁.a g₁ h₁ h₂).s = (playAMoveAt' g₂.a g₂ h₃ h₄).s ↔
+applyAMove g₁.s (g₁.a.f g₁.s h₁ h₂).m = applyAMove g₂.s (g₂.a.f g₂.s h₃ h₄).m := by rfl
 
 @[simp]
 theorem Game.s_playDMoveAt_eq_iff {pw} {g₁ g₂ : Game pw} {h₁ h₂} :
@@ -386,7 +388,7 @@ theorem Game.d_play {pw} {g : Game pw} {n} : (g.play n).d = g.d := by
 @[simp]
 theorem State.board_finish {s : State} : s.finish.board = s.board := rfl
 
-theorem Game.s_playAMoveAt_eq_of {pw} {g₁ g₂ : Game pw} (h₁ : g₁.s.act ↔ g₂.s.act)
+theorem Game.s_playAMoveAt_eq_iff_of {pw} {g₁ g₂ : Game pw} (h₁ : g₁.s.act ↔ g₂.s.act)
 (h₂ : AHasValidMove pw g₁.s.board ↔ AHasValidMove pw g₂.s.board) : ∀ h₁ h₂ h₃ h₄,
 (playAMoveAt g₁).s = (playAMoveAt g₂).s ↔
 applyAMove g₁.s (g₁.a.f g₁.s h₁ h₂).m = applyAMove g₂.s (g₂.a.f g₂.s h₃ h₄).m := by
@@ -411,68 +413,370 @@ theorem Game.s_play_initGame_d_set_eq_of_ne {pw a d s s₁ dRef n}
   have H₁ : g₁.a = g.a; simp [←hg, ←hg₁]
   simp [playDMoveAt]
   rw! [ih]
-  suffices h₂ : applyDMove g.s (g₁.d.f g.s h₁).m = applyDMove g.s (g.d.f g.s h₁).m
-  · rw [h₂]
-    generalize h₃ : applyDMove g.s (g.d.f g.s h₁).m = s'
-    have h₄ : s'.act; simpa [←h₃]
-    by_cases h₅ : ¬AHasValidMove pw s'.board
-    · iterate 2 rw [playAMoveAt_eq_of_neg # by tauto];; simp
-    push_neg at h₅
-    have h₆ := @s_playAMoveAt_eq_of _ (g₁.setState s') (g.setState s')
-      (by simp) (by simp) (by simpa) (by simpa) (by simpa) (by simpa)
-    rw [h₆]; clear h₆
-    simp; grind
-  congr 2; simp [←hg₁, D.set]
-  rw [if_neg]; simp [←hg]
-  rw [←hg]; apply h; omega
+  have h₂ : applyDMove g.s (g₁.d.f g.s h₁).m = applyDMove g.s (g.d.f g.s h₁).m
+  · congr 2; simp [←hg₁, D.set]
+    rw [if_neg]; simp [←hg]
+    rw [←hg]; apply h; omega
+  rw [h₂]
+  generalize h₃ : applyDMove g.s (g.d.f g.s h₁).m = s'
+  have h₄ : s'.act; simpa [←h₃]
+  by_cases h₅ : ¬AHasValidMove pw s'.board
+  · iterate 2 rw [playAMoveAt_eq_of_neg # by tauto];; simp
+  push_neg at h₅
+  have h₆ := @s_playAMoveAt_eq_iff_of _ (g₁.setState s') (g.setState s')
+    (by simp) (by simp) (by simpa) (by simpa) (by simpa) (by simpa)
+  rw [h₆]; clear h₆
+  simp; grind
 
--- theorem Game.s_play_eq_iff_of_act {pw} {g : Game pw} {n m}
--- (h : g.play (max n m) |>.act) : (g.play n).s = (g.play m).s ↔ n = m := by
---   sorry
+theorem Game.act_of_act_playMove {pw} {g : Game pw} (h : g.playMove.act) : g.act := by
+  by_contra h₁; simp [playMove, h₁] at h
+
+theorem Game.act_of_act_play {pw} {g : Game pw} {n} (h : (g.play n).act) : g.act := by
+  induction n; simp at h; exact h
+  nm n ih; apply ih
+  simp [play_succ] at h
+  exact act_of_act_playMove h
+
+@[simp]
+theorem State.length_history_applyAMove {s m} :
+(applyAMove s m).history.length = s.history.length + 1 := by
+  simp [applyAMove]
+
+@[simp]
+theorem State.length_history_applyDMove {s m} :
+(applyDMove s m).history.length = s.history.length + 1 := by
+  simp [applyDMove]
+
+@[simp]
+theorem Game.length_history_playAMoveAt' {pw} {g : Game pw} {a : A pw} {h₁ h₂} :
+(playAMoveAt' a g h₁ h₂).s.history.length = g.s.history.length + 1 := by
+  simp [playAMoveAt']
+
+@[simp]
+theorem Game.length_history_playDMoveAt {pw} {g : Game pw} {h} :
+(playDMoveAt g h).s.history.length = g.s.history.length + 1 := by
+  simp [playDMoveAt]
+
+@[simp]
+theorem State.history_finish {s : State} : s.finish.history = s.history := rfl
+
+theorem Game.length_history_playMove_eq_of_act {pw} {g : Game pw}
+(h : g.playMove.act) : g.playMove.s.history.length = g.s.history.length + 2 := by
+  have h₁ := act_of_act_playMove h
+  simp [h₁, playMove, playAMoveAt]
+  rw! (castMode := .all) [eq_true_of act_playDMoveAt, true_and]
+  rw [dif_pos]; simp
+  simp [playMove, h₁, playAMoveAt] at h
+  split_ifs at h with h₂ <;> simp_all
+
+theorem Game.length_history_play_eq_of_act {pw} {g : Game pw} {n}
+(h : (g.play n).act) : (g.play n).s.history.length = g.s.history.length + n * 2 := by
+  induction n; simp; nm n ih
+  simp [play_succ] at h ⊢
+  specialize ih # act_of_act_playMove h
+  rw [length_history_playMove_eq_of_act h]; omega
+
+@[simp]
+theorem Game.play_add {pw} {g : Game pw} {n m} : g.play (n + m) = (g.play n).play m := by
+  nth_rw 1 [play, add_comm]; rw [Function.iterate_add]; rfl
+
+theorem Game.s_play_eq_iff_of_act {pw} {g : Game pw} {n m}
+(h : g.play (max n m) |>.act) : (g.play n).s = (g.play m).s ↔ n = m := by
+  symm; constructor; rintro rfl; rfl
+  contrapose!
+  intro h₁
+  apply ne_of_congr (·.history.length)
+  wlog h₂ : n < m with ih; grind
+  clear h₁
+  rw [max_eq_right_of_lt h₂] at h
+  obtain ⟨m, rfl⟩ := Nat.exists_eq_add_of_le # le_of_lt h₂
+  simp at h ⊢
+  rw [length_history_play_eq_of_act h]; omega
+
+@[simp]
+theorem history_state₀ : state₀.history = [] := rfl
+
+@[simp]
+theorem Game.aTurn_playAMoveAt' {pw} {g : Game pw} {a : A pw} {h₁ h₂} :
+(playAMoveAt' a g h₁ h₂).s.aTurn = !g.s.aTurn := by
+  simp [playAMoveAt']
+
+theorem Game.aTurn_playMove_eq_of_act {pw} {g : Game pw}
+(h : g.playMove.act) : g.playMove.s.aTurn = g.s.aTurn := by
+  simp [playMove] at h ⊢
+  split_ifs at h ⊢ with h₁; on_goal 2 => contradiction
+  generalize hg₁ : playDMoveAt g h₁ = g₁ at h ⊢
+  have h₂ : g₁.act; simp [←hg₁]
+  simp [playAMoveAt] at h ⊢
+  rw! (castMode := .all) [eq_true_of h₂, true_and] at h ⊢
+  split_ifs at h ⊢ with h₃; on_goal 2 => simp at h
+  simp [←hg₁]
+
+theorem Game.aTurn_play_eq_of_act {pw} {g : Game pw} {n}
+(h : (g.play n).act) : (g.play n).s.aTurn = g.s.aTurn := by
+  induction n; simp; nm n ih; simp at h ⊢
+  specialize ih (act_of_act_playMove h)
+  rwa [aTurn_playMove_eq_of_act h]
+
+theorem aState_iff {pw s} : AState pw s ↔ s.WF pw ∧ s.aTurn = true := by
+  constructor <;> rintro ⟨⟩ <;> constructor <;> assumption
+
+theorem dState_iff {pw s} : DState pw s ↔ s.WF pw ∧ s.aTurn = false := by
+  constructor <;> rintro ⟨⟩ <;> constructor <;> assumption
+
+@[simp, instance]
+theorem aState_playDMoveAt {pw} {g : Game pw} {h}
+[hs : DState pw g.s] : AState pw (playDMoveAt g h).s := by
+  rw [dState_iff] at hs; choose hs ht using hs; rw [aState_iff]
+  rw [State.wf_iff] at hs ⊢
+  symm; split_ands; simpa
+  choose a d n g₁ h₁ h₂ using hs
+  symm at h₂; rcases h₂ with ⟨h', h₂⟩ | h₂
+  · contrapose h₂; clear h₂
+    apply ne_of_congr (·.aTurn)
+    simp [ht]
+    rw [←h₁] at h' ⊢
+    simp [Game.aTurn_play_eq_of_act h']
+  have h₃ : g₁.s.act
+  · replace h₂ := congrArg (·.aTurn) h₂
+    simp [ht] at h₂
+    apply Game.act_play_initGame_of_not_aTurn _ _ h₁ <;> simp_all
+  generalize hg' : (initGame a (d.set g₁.s g.d) state₀).play n = g'
+  refine' ⟨a, _, n, g', hg', _⟩; right
+  have h₄ : g'.s = g.s
+  · rw [←h₂, ←h₁, ←hg']
+    apply Game.s_play_initGame_d_set_eq_of_ne
+    intro k hk
+    simp [←h₁]
+    rw [Game.s_play_eq_iff_of_act]; omega
+    rw [max_eq_right_of_lt hk, h₁]
+    exact h₃
+  simp [h₄, h, applyDMove, applyMove]
+  congr 1; simp [←hg', D.set]; grind
+
+theorem Game.playAMoveAt_eq_of_not_act {pw} {g : Game pw}
+(h : ¬g.act) : playAMoveAt g = g.finish := by
+  simp [playAMoveAt, h]
+
+theorem Game.s_play_initGame_a_set_eq_of_ne {pw a d s s₁ aRef n}
+(h : ∀ k < n, ∀ h, (playDMoveAt (initGame a d s |>.play k) h : Game pw).s ≠ s₁) :
+(initGame (a.set s₁ aRef) d s |>.play n).s = (initGame a d s |>.play n).s := by
+  induction n; simp
+  nm n ih
+  specialize ih # by grind
+  simp [play_succ, playMove, act]
+  rw! (castMode := .all) [ih]
+  split_ifs with h₁
+  on_goal 2 => exact ih
+  generalize hg : (initGame a d s).play n = g at *
+  generalize hg₁ : (initGame (a.set s₁ aRef) d s).play n = g₁ at *
+  generalize_proofs H₁
+  generalize hgx : playDMoveAt g₁ H₁ = gx
+  generalize hgy : playDMoveAt g h₁ = gy
+  have H₂ : gx.s = gy.s
+  · subst hgx hgy
+    simp
+    congr 1
+    simp [←hg₁, ←hg]
+    rw! [ih]
+    rfl
+  simp [playAMoveAt, act]
+  rw! (castMode := .all) [H₂]
+  split_ifs with H₃; on_goal 2 => simp [H₂]
+  rcases H₃ with ⟨H₃, H₄⟩
+  simp
+  have H₅ : gx.a = a.set s₁ aRef; simp [←hgx, ←hg₁]
+  have H₆ : gy.a = a; simp [←hgy, ←hg]
+  rw! [H₅, H₆, ←H₂]
+  congr 2
+  simp [A.set]
+  contrapose!; rintro - rfl
+  contrapose h; clear h
+  simp
+  use n, by rfl
+  simp [hg, h₁, hgy, H₂]
+
+theorem Game.playAMoveAt_eq_of_pos {pw} {g : Game pw}
+(h₁ : g.act) (h₂ : AHasValidMove pw g.s.board) :
+playAMoveAt g = playAMoveAt' g.a g h₁ h₂ := by
+  simp [playAMoveAt, h₁, h₂]
+
+theorem Game.act_of_act_playAMoveAt {pw} {g : Game pw} (h : playAMoveAt g |>.act) : g.act := by
+  by_contra! h₁; simp [playAMoveAt, h₁] at h
+
+theorem Game.aHasValidMove_of_act_playAMoveAt {pw} {g : Game pw}
+(h : playAMoveAt g |>.act) : AHasValidMove pw g.s.board := by
+  by_contra! h₁; simp [playAMoveAt, h₁] at h
+
+theorem Game.s_playAMoveAt_eq_iff_of_act_playAMoveAt {pw} {g₁ g₂ : Game pw}
+(h₁ : playAMoveAt g₁ |>.act) (h₂ : playAMoveAt g₂ |>.act) :
+(playAMoveAt g₁).s = (playAMoveAt g₂).s ↔ applyAMove g₁.s (g₁.a.f g₁.s
+(act_of_act_playAMoveAt h₁) (aHasValidMove_of_act_playAMoveAt h₁)).m =
+applyAMove g₂.s (g₂.a.f g₂.s (act_of_act_playAMoveAt h₂)
+(aHasValidMove_of_act_playAMoveAt h₂)).m := by
+  have H₁ := act_of_act_playAMoveAt h₁
+  have H₂ := act_of_act_playAMoveAt h₂
+  have H₃ := aHasValidMove_of_act_playAMoveAt h₁
+  have H₄ := aHasValidMove_of_act_playAMoveAt h₂
+  simp [playAMoveAt]; rw [dif_pos ⟨H₁, H₃⟩, dif_pos ⟨H₂, H₄⟩]; simp
+
+@[simp]
+theorem Game.act_playAMoveAt' {pw} {g : Game pw} {a : A pw} {h₁ h₂} :
+(playAMoveAt' a g h₁ h₂).act ↔ g.act := by rfl
+
+theorem State.finish_eq_of_not_act {s : State} (h : ¬s.act) : s.finish = s := by
+  ext:1 <;> simp_all
+
+theorem Game.finish_eq_of_not_act {pw} {g : Game pw} (h : ¬g.act) : g.finish = g := by
+  ext:1 <;> simp; exact State.finish_eq_of_not_act h
+
+@[simp, instance]
+theorem dState_state₀ {pw} : DState pw state₀ := by
+  simp [dState_iff, State.wf_iff]; use default, default, 0; simp
+
+@[simp]
+theorem AState.aTurn {pw : outParam ℕ} {s} [hs : AState pw s] : s.aTurn = true := hs.ht
+
+@[simp]
+theorem DState.aTurn {pw : outParam ℕ} {s} [hs : DState pw s] : s.aTurn = false := hs.ht
+
+@[simp, instance]
+theorem wf_playAMoveAt {pw} {g : Game pw}
+[hs : AState pw g.s] : (playAMoveAt g).s.WF pw := by
+  rw [aState_iff] at hs; choose hs ht using hs
+  by_cases h : ¬g.s.act
+  · rw [Game.playAMoveAt_eq_of_neg # by tauto]
+    simpa [State.finish_eq_of_not_act h]
+  push_neg at h
+  rw [State.wf_iff] at hs ⊢
+  choose a d n g₁ h₁ h₂ using hs
+  rcases h₂ with h₂ | ⟨h', h₂⟩
+  · have h₀ : g₁.act; simpa [Game.act, h₂]
+    contrapose h₂; clear h₂
+    apply ne_of_congr (·.aTurn)
+    simp [ht]
+    rw [←h₁]
+    rw [Game.aTurn_play_eq_of_act]; simp
+    simpa [h₁]
+  generalize hg₀ : (initGame (a.set g.s g.a) d state₀).play n = g₀
+  generalize hg' : (initGame (a.set g.s g.a) d state₀).play (n + 1) = g'
+  refine' ⟨_, d, n + 1, g', hg', _⟩; left
+  have h₄ : g₀.s = g₁.s
+  · rw [←hg₀, ←h₁]
+    apply Game.s_play_initGame_a_set_eq_of_ne
+    intro k hk H₁
+    apply ne_of_congr (·.history.length)
+    simp [←h₂, ←h₁]
+    rw [Game.length_history_play_eq_of_act H₁]
+    rw [Game.length_history_play_eq_of_act # by rwa [h₁]]
+    simp; omega
+  simp [hg₀] at hg'
+  have h₀ : g₀.act; simpa [Game.act, h₄]
+  generalize hgx : playAMoveAt g = gx
+  generalize hgy : playDMoveAt g₀ h₀ = gy
+  replace hg' : playAMoveAt gy = g'
+  · rw [←hg']; simp [Game.playMove, h₀, hgy]
+  have Hd₀ : g₀.d = d; simp [←hg₀]
+  have Hd₁ : g₁.d = d; simp [←h₁]
+  have H₁ : gy.s = g.s
+  · simp [←hgy, ←h₂, Hd₀, Hd₁]; rw! [h₄]; rfl
+  have H₂ : gy.act; simp [←hgy]
+  by_cases H₃ : ¬AHasValidMove pw g.s.board
+  · rw [←hg', Game.playAMoveAt_eq_of_neg # by grind]
+    rw [←hgx, Game.playAMoveAt_eq_of_neg # by grind]
+    simp [H₁]
+  push_neg at H₃
+  have H₄ : g'.act
+  · simp [←hg']
+    rw [Game.playAMoveAt_eq_of_pos H₂ # by grind]
+    simpa [playAMoveAt']
+  have H₅ : gx.act
+  · rw [←hgx]; rwa [Game.playAMoveAt_eq_of_pos h H₃]
+  simp [←hg', ←hgx]
+  rw [Game.s_playAMoveAt_eq_iff_of_act_playAMoveAt (by grind) (by grind)]
+  rw! [H₁]; congr 2; simp [←hgy, ←hg₀, A.set]
+
+@[simp, instance]
+theorem Game.wf_playMove {pw} {g : Game pw}
+[hs : DState pw g.s] : g.playMove.s.WF pw := by
+  simp [playMove]; split_ifs <;> infer_instance
+
+theorem Game.playAMoveAt_eq_of_act {pw} {g : Game pw}
+(h : (playAMoveAt g).act) : playAMoveAt g = playAMoveAt' g.a g
+(act_of_act_playAMoveAt h) (aHasValidMove_of_act_playAMoveAt h) := by
+  simp [playAMoveAt, act_of_act_playAMoveAt h, aHasValidMove_of_act_playAMoveAt h]
+
+theorem Game.aTurn_playAMoveAt_of_act {pw} {g : Game pw}
+(h : (playAMoveAt g).act) : (playAMoveAt g).s.aTurn = !g.s.aTurn := by
+  simp [playAMoveAt_eq_of_act h]
+
+theorem dState_playAMoveAt_of_act {pw} {g : Game pw} [hs : AState pw g.s]
+(h : (playAMoveAt g).s.act) : DState pw (playAMoveAt g).s := by
+  constructor; rw [Game.aTurn_playAMoveAt_of_act h]; simp [hs.ht]
+
+theorem Game.dState_playMove_of_act {pw} {g : Game pw}
+[hs : DState pw g.s] (h : g.playMove.act) : DState pw g.playMove.s := by
+  constructor; rw [aTurn_playMove_eq_of_act h, hs.ht]
+
+@[simp, instance]
+theorem Game.wf_play {pw} {g : Game pw} {n} [hs : DState pw g.s] : (g.play n).s.WF pw := by
+  induction n; simp; infer_instance
+  nm n ih; simp; by_cases h₁ : (g.play n).s.act
+  · suffices : DState pw (g.play n).s; infer_instance
+    constructor; rw [aTurn_play_eq_of_act h₁, hs.ht]
+  rwa [playMove_eq_of_not_act h₁]
+
+theorem Game.dState_play_of_act {pw} {g : Game pw} {n}
+[hs : DState pw g.s] (h : (g.play n).act) : DState pw (g.play n).s := by
+  constructor; rw [aTurn_play_eq_of_act h, hs.ht]
+
+theorem not_dHws_of_aHws {pw} (h : AHws pw) : ¬DHws pw := by
+  obtain ⟨a, h⟩ := h; simp [DHws, DHwsAt]
+  intro d; use a; specialize h d; exact h
+
+theorem not_aHws_of_dHws {pw} (h : DHws pw) : ¬AHws pw := by
+  contrapose! h; exact not_dHws_of_aHws h
+
+@[simp, instance]
+theorem State.wf_toAltH_state₀ {pw} : sys.WF # state₀.toAltH pw := by
+  simp
+
+@[simp, instance]
+theorem State.wf_getd_toAltH?_state₀ {pw} : sys.WF # state₀.toAltH? pw |>.getd :=
+  wf_toAltH_state₀
+
+-- theorem Game.toAltH_playDMoveAt {pw} {g : Game pw} {h} [hs : DState pw g.s] :
+-- ∃ hist s', (g.s.toAltH pw).dMove (Point.toAlt # g.d.f g.s h) = some s' ∧
+-- (playDMoveAt g h).s.toAltH pw = s'.setHist hist
 
 -- #check 0 #exit
 
--- theorem wf_playDMoveAt {pw} {g : Game pw} {h} (hs : g.s.WF pw)
--- (ht : g.s.aTurn = false) : (playDMoveAt g h).s.WF pw := by
---   rw [State.wf_iff] at hs ⊢
---   choose a d n g₁ h₁ h₂ using hs
---   rcases h₂ with h₂ | ⟨h₂, h₃⟩
+-- @[simp, instance]
+-- theorem State.wf_toAltH {pw} {s : State} [hs : s.WF pw] : sys.WF # s.toAltH pw := by
+--   rw [wf_iff] at hs
+--   choose a d n g h₁ h₂ using hs
+--   induction n generalizing g
 --   ·
---     generalize hg' : (initGame a (d.set g₁.s g.d) state₀).play n = g'
---     refine' ⟨a, _, n, g', hg', _⟩
---     have h₃ : g₁.s.act
---     ·
---       replace h₂ := congrArg (·.aTurn) h₂
---       simp [ht] at h₂
---       apply Game.act_play_initGame_of_not_aTurn _ _ h₁ <;> simp_all
---     right
---     have h₄ : g'.s = g.s
---     ·
---       -- rw [←h₂, ←hg', ←h₁]
---       rw [←h₂, ←h₁, ←hg']
---       apply Game.s_play_initGame_d_set_eq_of_ne
---       intro k hk
---       simp [←h₁]
---       rw [Game.s_play_eq_iff_of_act]; omega
---       rw [max_eq_right_of_lt hk, h₁]
---     simp [h₄, h]
---     simp [applyDMove, applyMove]
---     congr 1
---     simp [←hg']
---     simp [D.set]
---     grind
---   ·
---     sorry
+--     simp at h₁
+--     simp [←h₁] at h₂
+--     rcases h₂ with rfl | ⟨h', h₂⟩; simp
+
+-- #check 0 #exit
+
+-- theorem Game.toAltH_playDMoveAt {pw} {g : Game pw} {h} [hs : DState pw g.s]
+-- (playDMoveAt g h).s.toAltH pw = (g.s.toAltH pw)
 
 -- #check 0 #exit
 
 -- theorem dHws_and_dwn_lt_toAltH_playDMoveAt_dOptimal_of_dHws {pw} {g g₁ : Game pw} {h}
+-- [hs : DState pw g.s]
 -- (h₁ : g.d = (dOptimal pw).getd)
 -- (h₂ : g.s.toAltH pw |>.dHws)
--- (ht : g.s.aTurn = false)
 -- (hg₁ : playDMoveAt g h = g₁) :
 -- (g₁.s.toAltH pw).dHws ∧ g₁.s.dwn pw < g.s.dwn pw := by
---   sorry
+--   split_ands
+--   ·
+--     simp [←hg₁]
 
 -- #check 0 #exit
 
