Projects/Sokoban/MovableBoxConjecture/Alts.lean
@@ -1,0 +1,1 @@
+import Projects.Sokoban.MovableBoxConjecture.Alts.Alt1
