Projects/Sokoban/MovableBoxConjecture/Alts/Alt1.lean
@@ -1,0 +1,3 @@
+import Projects.Sokoban.MovableBoxConjecture.Alts.Alt1.Defs
+import Projects.Sokoban.MovableBoxConjecture.Alts.Alt1.Auxi
+import Projects.Sokoban.MovableBoxConjecture.Alts.Alt1.Equiv
