Projects/Sokoban/MovableBoxConjecture/Alts/Alt1/Auxi.lean
@@ -1,0 +1,3 @@
+import Projects.Sokoban.MovableBoxConjecture.Alts.Alt1.Defs
+
+namespace Sokoban.MovableBoxConjecture.Alt₁
