Projects/Sokoban/MovableBoxConjecture/Alts/Alt1/Defs.lean
@@ -1,0 +1,32 @@
+import Projects.Sokoban.MovableBoxConjecture.Defs
+
+namespace Sokoban.MovableBoxConjecture.Alt₁
+
+open State
+
+inductive Tile where
+| Floor | Player | Box | Wall
+deriving DecidableEq open Tile
+
+structure State where
+  get : ℤ × ℤ → Tile
+  finite : {p | get p ≠ Wall}.Finite
+  player : ∃! p, get p = Player
+
+structure Step (s t : State) where
+  (p d : ℤ × ℤ)
+  dist : |d.1| + |d.2| = 1
+  player₁ : s.get p = Player
+  player₂ : t.get (p + d) = Player
+  floor : t.get p = Floor
+  box : if s.get (p + d) = Box
+    then s.get (p + d * 2) = Floor ∧ t.get (p + d * 2) = Box
+    else s.get (p + d) = Floor ∧ s.get (p + d * 2) = t.get (p + d * 2)
+  congr : ∀ q (k : Fin 3), q ≠ p + d * k → s.get p = t.get p
+
+inductive Reachable : State → State → Prop where
+| refl {s} : Reachable s s
+| step {s t t'} : Reachable s t → Step t t' → Reachable s t'
+
+def Conjecture : Prop :=
+  ∃ s, ∀ t, Reachable s t → ∃ t' p, Reachable t t' ∧ t.get p = Box ↔ t'.get p ≠ Box
